Completed sketch proof, we might need RC between S and I.

Common/Rc.v
@@ -15,20 +15,23 @@ Require Import Coq.Program.Basics.
  *)
 
 (* Component id *)
-Variable id : Type.
+Axiom id : Type.
 Definition interface := list id.
 (* check if the last event of a behavior belongs to an agent,
    represented by the interface of its components *)
-Variable turn : program_behavior -> interface -> Prop.
+Axiom turn : program_behavior -> interface -> Prop.
 (* check if an interface is complete *)
-Variable icomplete : interface -> Prop.
+Axiom icomplete : interface -> Prop.
 (* check if the union of two interfaces is complete *)
 Definition icomplete2 (i1 i2:interface) := icomplete (i1++i2).
-(* Hypothesis unique_interfaces : *)
-(*   forall (i1 i2 i3:interface), *)
-(*     icomplete2 i1 i3 -> icomplete2 i2 i3 -> i1=i2. *)
+(* TODO check this *)
+Axiom unique_interfaces :
+  forall (i1 i2 i3:interface),
+    icomplete2 i1 i3 -> icomplete2 i2 i3 -> i1=i2.
 
-
+(* 
+   option monad stuff
+ *)
 Definition map {A B} (f: A -> B) (o: option A) : option B :=
   match o with
   | Some a => Some (f a)
@@ -48,6 +51,7 @@ Definition behaves (o: option semantics) b :=
     | None => False
     end.
 
+
 (* 
    The languages.
  *)
@@ -55,27 +59,27 @@ Definition behaves (o: option semantics) b :=
 (* Signature of basic things expected in a language *)
 Module Type Lang.
   (* Type of programs, complete or partial *)
-  Variable program : Type.
-  Variable get_interface: program -> interface.
+  Axiom program : Type.
+  Axiom get_interface: program -> interface.
   (* checks if a program has a complete interface *)
-  Variable complete: program -> Prop.
+  Axiom complete: program -> Prop.
   (* checks if two programs linked together form a complete program *)
-  Variable complete2: program -> program -> Prop.
+  Axiom complete2: program -> program -> Prop.
 
   (* complete semantics: takes a complete program *)
-  Variable sem: option program -> option semantics.
-  (* Variable sem_complete: *)
+  Axiom sem: option program -> option semantics.
+  (* Axiom sem_complete: *)
   (*   forall (p:program), *)
   (*     complete p -> exists s, sem (Some p) = Some s. *)
 
   (* partial semantics: takes a program and a matching interface.
      The interface of the program together with the matching interface
      is complete. *)
-  Variable psem: option program -> interface -> option semantics.
-  (* Variable psem_complete: *)
+  Axiom psem: option program -> interface -> option semantics.
+  (* Axiom psem_complete: *)
   (*   forall psi (p:program), *)
   (*     icomplete2 psi (get_interface p) -> exists s, psem (Some p) psi = Some s. *)
-  (* Variable idefinability: forall (i:interface), exists (p:program), get_interface p = i. *)
+  (* Axiom idefinability: forall (i:interface), exists (p:program), get_interface p = i. *)
 End Lang.
 
 (* Every language is a subtype of Lang and implements its signature *)
@@ -83,40 +87,65 @@ End Lang.
 
 (* Target *)
 Module T <: Lang.
-  Variable program : Type.
-  Variable get_interface: program -> interface.
+  Axiom program : Type.
+  Axiom get_interface: program -> interface.
   Definition complete (p:program) := icomplete (get_interface p).
   Definition complete2 (p1 p2:program) := icomplete2 (get_interface p1) (get_interface p2).
-  Variable sem: option program -> option semantics.
-  Variable psem: option program -> interface -> option semantics.
+  Axiom sem: option program -> option semantics.
+  Axiom psem: option program -> interface -> option semantics.
+
+  (* takes a complete program and produces a partial one
+   This is an important ingredient for the simulation relation.
+   For MP the relation corresponds with this function actually.
+   For SFI the relation contains additional elements.
+   *)
+  Axiom partialize: interface -> T.program -> T.program.
+  (* Axiom partialize_post: *)
+  (*   forall (p pp:T.program) psi, *)
+  (*   partialize psi p = pp -> *)
+  (*   (T.get_interface p) = (T.get_interface pp)++psi. *)
 End T.
 
 (* Intermediate *)
 Module I <: Lang.
-  Variable program : Type.
-  Variable get_interface: program -> interface.
+  Axiom program : Type.
+  Axiom get_interface: program -> interface.
   Definition complete (p:program) := icomplete (get_interface p).
   Definition complete2 (p1 p2:program) := icomplete2 (get_interface p1) (get_interface p2).
-  Variable sem: option program -> option semantics.
-  Variable psem: option program -> interface -> option semantics.
+  Axiom sem: option program -> option semantics.
+  Axiom psem: option program -> interface -> option semantics.
 
   (* linking of two partial programs, returns a complete program *)
-  Variable link: program -> program -> option program.
+  Axiom link: program -> program -> option program.
+  Axiom link_prepost:
+    forall (p1 p2:program),
+      complete2 p1 p2 -> exists p, (link p1 p2 = Some p) /\ (get_interface p = (get_interface p1) ++ (get_interface p2)).
+
+  Axiom decomposition:
+    forall beh (c p:I.program),
+      behaves (I.sem (I.link c p)) beh
+      ->
+      behaves (I.psem (Some p) (I.get_interface c)) beh.
+
+  Definition fully_defined (psi:interface) (p:program) :=
+    forall (beh:program_behavior) (c:program),
+      get_interface c = psi ->
+      complete2 c p ->
+      behaves (sem (link c p)) beh ->
+      (turn beh (get_interface p) ->
+      not_wrong beh).
 End I.
 
 (* Source *)
 Module S <: Lang.
-  Variable program : Type.
-  Variable get_interface: program -> interface.
+  Axiom program : Type.
+  Axiom get_interface: program -> interface.
   Definition complete (p:program) := icomplete (get_interface p).
   Definition complete2 (p1 p2:program) := icomplete2 (get_interface p1) (get_interface p2).
-  Variable sem: option program -> option semantics.
-  Variable psem: option program -> interface -> option semantics.
+  Axiom sem: option program -> option semantics.
+  Axiom psem: option program -> interface -> option semantics.
 
-  Variable link: program -> program -> option program.
-  (* Variable link_prepost: *)
-  (*   forall (p1 p2 p:program), *)
-  (*     complete2 p1 p2 -> (link p1 p2 = Some p) /\ (get_interface p = (get_interface p1) ++ (get_interface p2)). *)
+  Axiom link: program -> program -> option program.
 
   Definition fully_defined (psi:interface) (p:program) :=
     forall (beh:program_behavior) (c:program),
@@ -126,7 +155,7 @@ Module S <: Lang.
       (turn beh (get_interface p) ->
       not_wrong beh).
 
-  Hypothesis definability:
+  Axiom definability:
     forall (beh:program_behavior) (psi:interface) (p:program),
       icomplete2 psi (get_interface p) ->
       behaves (psem (Some p) psi) beh ->
@@ -138,12 +167,12 @@ End S.
 (* This module takes a high language L1 and a low one L2 and produces
    a compiler from L1 to L2 and some properties *)
 Module Compiler (L1 L2: Lang).
-  Variable compile : L1.program -> L2.program.
-  Hypothesis compile_complete :
+  Axiom compile : L1.program -> L2.program.
+  Axiom compile_complete :
     forall p1 p2,
       L1.complete p1 -> compile p1 = p2 -> L2.complete p2.
   
-  Hypothesis compiler_interfaces:
+  Axiom compiler_interfaces:
   forall (p1:L1.program),
     L1.get_interface p1 = L2.get_interface (compile p1).
 End Compiler.
@@ -151,12 +180,86 @@ End Compiler.
 Module IT := Compiler I T.
 Module SI := Compiler S I.
 
-(* Hypothesis Tnotwrong : *)
-(*   forall b p, *)
-(*     program_behaves (T.sem p) b -> not_wrong b. *)
-(* Hypothesis Tpnotwrong : *)
-(*   forall b p psi, *)
-(*     program_behaves (T.psem p psi) b -> not_wrong b. *)
+(* TODO IT.compile must be a refinement compiler *)
+
+(* exact cc preserves also UB *)
+Axiom SIcompiler_correctness :
+  forall beh (p:S.program) (psi:interface),
+    behaves (I.psem (Some (SI.compile p)) psi) beh ->
+    behaves (S.psem (Some p) psi) beh.
+
+
+(* Warm-up: RC between S and I *)
+Definition SIrc:
+  forall (c:I.program) (P:S.program) (beh:program_behavior),
+    icomplete2 (I.get_interface c) (S.get_interface P) ->
+    S.fully_defined (I.get_interface c) P ->
+    behaves (I.sem (I.link c (SI.compile P))) beh
+    ->
+    exists C,
+      behaves (S.sem (S.link C P)) beh /\ S.complete2 C P.
+Proof.
+  intros c P b Hcomplete SFD H.
+  apply I.decomposition in H.
+  destruct (I.link_prepost c (SI.compile P)) as [p [H1 H2]].
+  unfold I.complete2.
+  rewrite <- SI.compiler_interfaces.
+  auto.
+  apply (SIcompiler_correctness b P (I.get_interface c)) in H.
+  apply S.definability in H.
+  destruct H as [C [Hb Hif]].
+  exists C.
+  split.
+  auto.
+  rewrite <- Hif in Hcomplete.
+  auto.
+  auto.
+Qed.
+
+
+
+(* 
+   We now got for RC between S and T.
+   The following properties are special because they depend on
+   compiling the complete intermediate program.
+ *)
+Axiom Tspecial_decomposition:
+  forall beh (c p:I.program),
+    let ip := map IT.compile (I.link c p) in
+    behaves (T.sem ip) beh
+    ->
+    behaves (T.psem (map (T.partialize (I.get_interface c)) ip) (I.get_interface c)) beh.
+
+Axiom ITspecial_compiler_correctness:
+  forall beh (c p:I.program),
+    I.fully_defined (I.get_interface c) p ->
+    let ip := I.link c p in
+    let tp := map (T.partialize (I.get_interface c)) (map IT.compile ip) in
+    behaves (T.psem tp (I.get_interface c)) beh ->
+    behaves (I.psem (Some p) (I.get_interface c)) beh.
+
+(* This is proved using SIrc. *)
+Definition FD_preservation:
+  forall (psi:interface) (p:S.program),
+  S.fully_defined psi p ->
+  I.fully_defined psi (SI.compile p).
+Proof.
+  intros psi p SFD.
+  intros b c Hpsi Hcomplete H1.
+  unfold I.complete2 in Hcomplete.
+  rewrite <- SI.compiler_interfaces in Hcomplete.
+  destruct (SIrc c p b Hcomplete) as [C [H2 H3]].
+  rewrite Hpsi.
+  apply SFD.
+assumption.
+  unfold S.fully_defined in SFD.
+  rewrite <- SI.compiler_interfaces.
+  apply (SFD b C).
+  unfold S.complete2 in H3.  
+  destruct (unique_interfaces (I.get_interface c) (S.get_interface C) (S.get_interface p)); auto.
+auto.
+auto.
+Qed.
 
 (* 
    This property is different from the one we started from: there is
@@ -176,6 +279,22 @@ Definition robust_compilation_static_compromise :=
     exists C, 
       behaves (S.sem (S.link C P)) beh /\ S.complete2 C P.
 
+Theorem proof_rc_static : robust_compilation_static_compromise.
+Proof.
+  intros c P b Hcomplete SFD H.
+  apply (Tspecial_decomposition b c (SI.compile P)) in H.
+  apply ITspecial_compiler_correctness in H.
+  destruct (S.definability b (I.get_interface c) P Hcomplete) as [C [H1 Hinterfaces]].
+  apply (SIcompiler_correctness b P (I.get_interface c)) in H.
+  assumption.
+  rewrite <- Hinterfaces in Hcomplete.
+  exists C.
+  auto.
+  apply FD_preservation.
+  assumption.
+Qed.
+
+
 (* This definition is weaker than the above but has the advantage of
    not mentioning the intermediate language *)
 Definition robust_compilation_static_compromise_corollary :=
@@ -186,8 +305,8 @@ Definition robust_compilation_static_compromise_corollary :=
     behaves (T.sem (map compile (S.link Q P))) beh ->
     exists C, behaves (S.sem (S.link C P)) beh /\ S.complete2 C P.
 
-(* This is too syntactic, it should be stated in terms of equivalent behaviors *)
-Hypothesis Sseparate_compilation:
+(* TODO This is too syntactic, it should be stated in terms of equivalent behaviors *)
+Axiom Sseparate_compilation:
   forall (P Q: S.program),
     map SI.compile (S.link Q P) = I.link (SI.compile Q) (SI.compile P).
 
@@ -202,54 +321,4 @@ Proof.
   rewrite <- Sseparate_compilation in RC.
   rewrite <- map_compose in H3.  
   apply (RC Hcompl H1 H3).
-Qed.
-
-
-(* Extra ingredients needed for the proof. *)
-
-(* takes a complete program and produces a partial one
-   This is an important ingredient for the simulation relation.
-   For MP the relation corresponds with this function actually.
-   For SFI the relation contains additional elements.
- *)
-Variable Tpartialize: interface -> T.program -> T.program.
-(* Hypothesis partialize_post: *)
-(*   forall (p pp:T.program) psi, *)
-(*   Tpartialize psi p = pp -> *)
-(*   (T.get_interface p) = (T.get_interface pp)++psi. *)
-
-Hypothesis Tdecomposition:
-  forall beh (c p:I.program),
-    let ip := map IT.compile (I.link c p) in
-    behaves (T.sem ip) beh
-    ->
-    behaves (T.psem (map (Tpartialize (I.get_interface c)) ip) (I.get_interface c)) beh.
-
-(* TODO IT.compile must be a refinement compiler *)
-
-Hypothesis ITspecial_pcompiler_correctness:
-  forall beh (c p:I.program),
-    (* I.fully_defined (I.get_interface c) p -> *)
-    let ip := I.link c p in
-    let tp := map (Tpartialize (I.get_interface c)) (map IT.compile ip) in
-    behaves (T.psem tp (I.get_interface c)) beh ->
-    behaves (I.psem (Some p) (I.get_interface c)) beh.
-
-(* exact cc preserves also UB *)
-Hypothesis SIpcompiler_correctness :
-  forall beh (p:S.program) (psi:interface),
-    behaves (I.psem (Some (SI.compile p)) psi) beh ->
-    behaves (S.psem (Some p) psi) beh.
-
-Theorem proof_rc_static : robust_compilation_static_compromise.
-Proof.
-  intros c P b Hcomplete SFD H.
-  apply (Tdecomposition b c (SI.compile P)) in H.
-  apply ITspecial_pcompiler_correctness in H.
-  destruct (S.definability b (I.get_interface c) P Hcomplete) as [C [H1 Hinterfaces]].
-  apply (SIpcompiler_correctness b P (I.get_interface c)) in H.
-  assumption.
-  rewrite <- Hinterfaces in Hcomplete.
-  exists C.
-  auto.
 Qed.
